# 1.4 Exact ODEs. Integrating Factors

If a function a function $u(x,y)$ has continuous partial derivatives, its **differential** is:

$$du = \frac{\partial u }{\partial x}dx + \frac{\partial u}{\partial y}dy$$

It is trivial to show that if $u(x,y) = c = const$, then $du = 0$.

Here we will show via example that this differential of a constant function can be a manipulated form of an ODE.

$$u = x + x^2y^3 = c$$
$$du = (1 + 2xy^3)dx + 3x^2y^2dy = 0$$
$$(1 + 2xy^3)dx = -3x^2y^2dy$$
$$y' = \frac{dy}{dx} = -\frac{1 + 2xy^3}{3x^2y^2}$$

This is clearly the [[Explicit Form]] of a [[First-Order ODE]], and this manipulation leads us to a powerful solution method for linear first-order ODEs... 

A first-order ODE $M(x,y) + N(x,y)y' = 0$, written as

> $$M(x,y)dx + N(x,y)dy = 0 \tag{1}$$

is referred to as an [[Exact Differential Equation]] under the condition that the **differential form** is **exact**.

What is the **differential form**? The differential form is the LHS of $(1)$.

What does it mean for the **differential form** to be **exact**? To be **exact**, $\eqref{2}$ must be the differential
> $$du = \frac{\partial u}{\partial x}dx + \frac{\partial u}{\partial y}dy \tag{2}$$

of some function $u(x,y)$, meaning $(1)$ can be written
$$du = 0$$

Integrating gives us the general solution of $(1)$ in the form
> $$u(x,y) = c \tag{3}$$

$(3)$ is called an [[Implicit Solution]] as opposed to an [[Explicit Solution]] of the form $y = h(x)$.

## Exact Differential Equation

Exact differential equations are extremeley convenient because as we showed above, it is simple to obtain an implicit solution via integration of $M(x,y)$ and/or $N(x,y)$.

Looking at $(1)$ and $(2)$ we can see that $(1)$ is an exact differential equation if there is some function $u(x,y)$ such that

1. $$\frac{\partial u}{\partial x} = M \tag{4a}$$
2. $$\frac{\partial u}{\partial y} = N \tag{4b}$$

To verify if an equation of the form in $(1)$ is an exact differential equation or not, we can perform the following check.

### Conditions for Exactness

> Let $M$ and $N$ be **continuous** and have **continuous first partial derivatives** in a region in the xy-plane whose boundary is a closed curve without self-intersections. Then by partial differentiaion of $(4)$:
> $$\frac{\partial M}{\partial y} = \frac{\partial^2 u}{\partial y \partial x}$$
> $$\frac{\partial N}{\partial x} = \frac{\partial^2 u}{\partial x \partial y}$$
> By the assumption of continuity the two second partial derivatives are equal. Thus
> $$\frac{\partial M}{\partial y} = \frac{\partial N}{\partial x} \tag{5}$$

This condition is necessary and sufficient for $(1)$ to be an exact differential equation.

### Solving the Exact Differential Equation

Integrate $(4a)$ with respect to $x$

> $$u = \int M dx + k(y) \tag{6}$$

Because $(4a)$ is a partial derivative of $u(x,y)$ with respect to $x$ we can integrate it treating $y$ as a constant and add a function of $y$, $k(y)$ to the result. We then take the partial derivative of $(6)$ with respect to $y$ and set this equal to $(4b)$ to get $dk/dy$, and integrate $dk/dy$ to get $k$.

We can do the same process starting with $(4b)$ instead.

> $$u = \int N dy + l(x) \tag{6*}$$

### An Example

Solve

$$cos(x + y)dx + (3y^2 + 2y + cos(x + y))dy = 0 \tag{7}$$

***Step 1. Test for exactness.***
$$M = cos(x + y)$$
$$N = 3y^2 + 2y + cos(x+y)$$
Both of these equations and their partial derivatives in the xy-plane are continuous, thus
$$\frac{\partial M}{\partial y} = -sin(x + y)$$
$$\frac{\partial N}{\partial x} = -sin(x + y)$$

***Step 2. Implicit general solution.***

$$u = \int M dx + k(y) = \int cos(x + y)dx + k(y) = sin(x + y) + k(y) \tag{8}$$
To find $k(y)$, differentiate with respect to $y$ and use formula $(4b)$
$$\frac{\partial u}{\partial y} = cos(x + y) + \frac{dk}{dy} = N = 3y^2 + 2y + cos(x + y)$$
$$dk/dy = 3y^2 + 2y$$
By integration
$$k = y^3 + y^2 + c*$$
Inserting into $(8)$ gives us the *answer*
$$u(x,y) = sin(x + y) + y^3 + y^2 = c$$

***Step 3. Checking an implicit solution***
Check out solution by differentiating the implicit solution $u(x, y) = c$ implicitly and see whether this leads to the given ODE $(7)$:
$$du = \frac{\partial u}{\partial x}dx + \frac{\partial u}{\partial y}dy = cos(x + y)dx + (cos(x + y) + 3y^2 + 2y)dy = 0$$